Safety: progress in assembly safety interface, using CA as the example

driver/CA.v
@@ -5,6 +5,7 @@ Require Import Conventions Mach Asm.
 Require Import CKLR.
 Require Import Locations CallConv.
 Require Import Inject InjectFootprint.
+Require Import MemFootprint.
 
 (*
    cc_c_asm_injp   ≡    c_injp @  ≡ c_injp @
@@ -202,38 +203,223 @@ Qed.
 
 (** Experiment code for flatening CAinjp into a safety interface *)
 
-Record inv_cainjp_world :=
-  inv_cajw {
-      inv_cajw_fp: Mem.sup;
-      inv_cajw_mem: mem;
-      inv_cajw_sg : signature;
-      inv_cajw_rs : regset;
+Record inv_asm_cc_injp_world :=
+  inv_asmcc_w {
+      inv_asmcc_fp: mem_valid_world;
+      inv_asmcc_sg: signature;
+      inv_asmcc_rs : regset;
     }.
 
+Local Open Scope mfp_scope.
+
 (** TODO: remove c_query, remove Hm, refine the sup  *)
-Inductive inv_c_asm_injp_mq : inv_cainjp_world -> c_query -> query li_asm -> Prop:=
-  inv_c_asm_injp_mq_intro sg args m sup (rs: regset) tm0 vf
-    (* TODO: write a more general condition *)
-    (Hm: Mem.inject (Mem.flat_inj sup) m m):
+(* Safety interface for asm query that contains the asm-level calling
+convention and the memory protection *)
+Inductive inv_asm_cc_injp_q : inv_asm_cc_injp_world -> query li_asm -> Prop:=
+  inv_asm_cc_injp_q_intro tm mfp (rs: regset) m0 sg
+    (Hm: memory_valid mfp tm):
     let tsp := rs#SP in let tra := rs#RA in let tvf := rs#PC in
-    let targs := (map (fun p => Locmap.getpair p (make_locset_rs rs m tsp))
+    let targs := (map (fun p => Locmap.getpair p (make_locset_rs rs tm tsp))
                     (loc_arguments sg)) in
-    (* TODO  *)
-    Val.inject_list (Mem.flat_inj sup) args targs ->
-    Val.inject (Mem.flat_inj sup) vf tvf ->
+    valid_val_list mfp targs ->
+    valid_val mfp tvf ->
     (forall b ofs, loc_init_args (size_arguments sg) tsp b ofs ->
-              loc_out_of_reach (Mem.flat_inj sup) m b ofs) ->
+              mfp ! b ## ofs = false) ->
     Val.has_type tsp Tptr ->
     Val.has_type tra Tptr ->
-    valid_blockv (Mem.support m) tsp ->
-    args_removed sg tsp m tm0 -> (* The Outgoing arguments are readable and freeable in tm *)
-    vf <> Vundef -> tra <> Vundef ->
-    inv_c_asm_injp_mq
-      (inv_cajw sup m sg rs)
+    valid_blockv (Mem.support tm) tsp ->
+    args_removed sg tsp tm m0 -> (* The Outgoing arguments are readable and freeable in tm *)
+    (* Do we actually need these? *)
+    tra <> Vundef ->
+    inv_asm_cc_injp_q
+      (inv_asmcc_w (mvw mfp tm Hm) sg rs)
+      (rs,tm).
+
+(* Convention of allocating registers for the C arguments *)
+Inductive cc_c_asm_args_q: signature -> query li_c -> query li_asm -> Prop :=
+  cc_c_asm_args_q_intro sg m (rs: regset) :
+    let tsp := rs#SP in let vf := rs#PC in
+    let args := (map (fun p => Locmap.getpair p (make_locset_rs rs m tsp))
+                      (loc_arguments sg)) in
+    vf <> Vundef -> 
+    cc_c_asm_args_q
+      sg
       (cq vf sg args m)
-      (rs,m).
+      (rs, m).
 
 
+(* Safety interface for asm reply that contains the asm-level calling
+convention and the memory protection *)
+Inductive inv_asm_cc_injp_r : inv_asm_cc_injp_world -> reply li_asm -> Prop :=
+  inv_asm_cc_injp_r_intro sg mfp tm Hm mfp' tm' Hm' (rs rs' :regset) :
+     let tsp := rs#SP in
+     let tres := rs_getpair (map_rpair preg_of (loc_result sg)) rs' in
+     valid_val mfp' tres ->
+     mvw_acc (mvw mfp tm Hm) (mvw mfp' tm' Hm') ->
+     (forall r, is_callee_save r = true -> rs' (preg_of r) = rs (preg_of r)) ->
+     rs'#SP = rs#SP -> rs'#PC = rs#RA ->
+     inv_asm_cc_injp_r
+       (inv_asmcc_w (mvw mfp tm Hm) sg rs)
+       (rs', tm').
+
+(* Convention of allocating registers for the C return value *)
+Inductive cc_c_asm_res_r: signature -> reply li_c -> reply li_asm -> Prop :=
+  cc_c_asm_res_r_intro sg m (rs: regset):
+    let res := rs_getpair (map_rpair preg_of (loc_result sg)) rs in
+    cc_c_asm_res_r
+      sg
+      (cr res m)
+      (rs, m).
+
+Definition inv_asm_cc_injp : invariant li_asm :=
+  {| inv_world := inv_asm_cc_injp_world;
+    symtbl_inv w se := mem_valid_stbl (inv_asmcc_fp w) se;
+    query_inv := inv_asm_cc_injp_q;
+    reply_inv := inv_asm_cc_injp_r; |}.
+
+Program Definition cc_c_asm_args_res : callconv li_c li_asm :=
+  {|
+    match_senv _ := eq;
+    match_query := cc_c_asm_args_q;
+    match_reply := cc_c_asm_res_r;
+  |}.
+Next Obligation.
+  split; intros; auto.
+Defined.
+
+Require Import InvariantAlgebra.
+
+Local Open Scope inv_scope.
+
+Definition meminj_inv : Type := (NMap.t (Maps.ZMap.t (option (block * Z)))).
+
+(* The inverse function of the memory injection *)
+Definition tm_inj (j: meminj) (m: mem) : meminj_inv :=
+  (NMap.init _ (Maps.ZMap.init None)).
+
+(** TODO: construct target footprint from the injection *)
+Definition tm_fp (j: meminj_inv) : memfp := 
+  NMap.map _ _ (fun zm => Maps.ZMap.map (fun elt => match elt with | Some _ => true | None => false end) zm) j.
+
+Lemma inject_implies_valid_memory: forall m tm j,
+    Mem.inject j m tm ->
+    memory_valid (tm_fp (tm_inj j m)) tm.
+Admitted.
+
+Lemma inject_implies_valid_val: forall v1 v2 j m,
+    Val.inject j v1 v2 ->
+    valid_val (tm_fp (tm_inj j m)) v2.
+Admitted.
+
+Lemma inject_implies_valid_val_list: forall vl1 vl2 j m,
+    Val.inject_list j vl1 vl2 ->
+    valid_val_list (tm_fp (tm_inj j m)) vl2.
+Admitted.
+
+Lemma tm_fp_out_of_reach: forall j m b ofs,
+    loc_out_of_reach j m b ofs ->
+    (tm_fp (tm_inj j m)) ! b ## ofs = false.
+Admitted.
+
+
+(** Construct the inverse injection *)
+
+(* TODO: one problem is how to find the largest consecutive memory
+regions for building a source block *)
+Definition tm_inj' (invj: meminj_inv) (tm tm': mem) (mfp': memfp) : meminj_inv :=
+  invj.
+
+(** Construct the outgoing source memory with the new inverse injection *)
+
+(* TODO: Iterate the tm' and construct memory values to update m *)
+Definition m'_from_invj' (invj': meminj_inv) (m tm': mem) : mem := m.
+
+(* top level theorem of the injp construction for outgoing reply *)
+Lemma mfp_outgoing_constr: forall j m tm (INJ: Mem.inject j m tm) Hm mfp' tm' Hm',
+    let invj := tm_inj j m in
+    let mfp := tm_fp invj in
+    mvw_acc (mvw mfp tm Hm) (mvw mfp' tm' Hm') ->
+    exists j' m' INJ',
+      injp_acc (injpw j m tm INJ) (injpw j' m' tm' INJ')
+      (* move this property to other places *)
+      /\ (forall v', valid_val mfp' v' -> 
+              exists v, Val.inject j' v v').
+Admitted.
+
+(* This property classifies those safety interfaces that are preserved
+up to the memory injeciton. It says that the safety interface is
+irrelavent to the injection (i.e., the name of the memory block) *)
+Record c_interface_up_to_inj (P: invariant li_c) : Prop :=
+  { c_interface_up_to_inj_incoming:
+    forall w1 args1 args2 vf1 vf2 m1 m2 sg j,
+      query_inv P w1 (cq vf1 sg args1 m1) ->
+      Mem.inject j m1 m2 ->
+      Val.inject j vf1 vf2 ->
+      Val.inject_list j args1 args2 ->
+      exists w2, query_inv P w2 (cq vf2 sg args2 m2)
+            /\ (forall vres1 vres2 m1' m2' j',
+                  reply_inv P w2 (cr vres2 m2') ->
+                  Mem.inject j' m1' m2' ->
+                  Val.inject j' vres1 vres2 ->
+                  reply_inv P w1 (cr vres1 m1'));
+    
+    c_interface_up_to_inj_outgoing:
+    forall w2 args1 args2 vf1 vf2 m1 m2 sg j,
+      query_inv P w2 (cq vf2 sg args2 m2) ->
+      Mem.inject j m1 m2 ->
+      Val.inject j vf1 vf2 ->
+      Val.inject_list j args1 args2 ->
+      exists w1, query_inv P w1 (cq vf1 sg args1 m1)
+            /\ (forall vres1 vres2 m1' m2' j',
+                  reply_inv P w1 (cr vres1 m1') ->
+                  Mem.inject j' m1' m2' ->
+                  Val.inject j' vres1 vres2 ->
+                  reply_inv P w2 (cr vres2 m2'));
+  }.
+    
+
+
+
+Lemma c_asm_inv_cainjp: forall P (UINJ: c_interface_up_to_inj P),
+    invref 
+      (P @! cc_c_asm_injp)
+      ((P @! cc_c_asm_args_res) @@ inv_asm_cc_injp).
+Proof.
+  intros. red.
+  intros (wP1 & wca) se2 q2 (se1 & SYM1 & MSENV) (q1 & QINV1 & MQ).
+  (** TODO: iterate over the ~loc_out_of_reach to construct mfp *)
+  destruct wca as [[j m tm Hm] sg rs]. 
+  (* construct wP2 *)
+  inv MQ.
+  exploit (c_interface_up_to_inj_incoming _ UINJ); eauto. intros (wP2 & QINV2 & RINV2). 
+  set (invj := tm_inj j m).
+  exists ((wP2, sg), inv_asmcc_w (mvw (tm_fp invj) tm (inject_implies_valid_memory m tm j Hm1)) sg rs). 
+  split. 2: split.
+  (* symbol table *)
+  - admit.
+  (* query *)
+  - econstructor.
+    + exists (cq tvf sg targs tm). split; eauto.
+      econstructor; eauto. fold tvf.
+      inv H5; subst; try congruence.
+    + econstructor. 4-8: eauto.
+      * eapply inject_implies_valid_val_list; eauto.
+      * eapply inject_implies_valid_val; eauto.
+      * intros. eapply tm_fp_out_of_reach; eauto.
+  - intros r2 ((r1 & (RINV1' & RINV2')) & RINV3').
+    inv RINV3'. inv RINV2'.
+    (** TODO: construct a source memory m' such that (m, tm) ~->_injp (m', tm') *)
+    exploit mfp_outgoing_constr; eauto. 
+    instantiate (1 := Hm1). intros (j' & m' & INJ' & INJP & VP).
+    (* construct source return value *)
+    exploit VP; eauto. intros (res1 & VINJ_RES).
+    exists (cr res1 m'). 
+    split.
+    + eapply RINV2; eauto. 
+    + inv INJP. econstructor; eauto.
+      econstructor; eauto.
+Admitted.
+        
 Lemma cc_injpca_cainjp :
   ccref (cc_c injp @ cc_c_asm) (cc_c_asm_injp).
 Proof.
